adds mode polymorphism and generalises ! τ and ¡ θ

theories/case_studies/c.v
@@ -27,11 +27,12 @@ From affect.logic Require Import tactics.
 
 (* Make all the definitions opaque so that we do not rely on their definition in the model to show that the programs are well-typed terms. *)
 Opaque sem_typed sem_typed_val ty_le row_le sig_le row_type_sub row_env_sub.
-Opaque sem_ty_void sem_ty_unit sem_ty_bool sem_ty_int sem_ty_string sem_ty_top sem_ty_cpy sem_env_cpy sem_ty_ref_cpy sem_ty_ref sem_ty_prod sem_ty_sum sem_ty_arr sem_ty_aarr sem_ty_uarr sem_ty_forall sem_ty_row_forall sem_ty_exists sem_ty_rec sem_ty_option sem_ty_list.
-Opaque sem_sig_eff sem_sig_os.
-Opaque sem_row_nil sem_row_os sem_row_cons sem_row_rec.
+Opaque sem_ty_void sem_ty_unit sem_ty_bool sem_ty_int sem_ty_string sem_ty_top sem_ty_bang sem_env_bang sem_ty_ref_cpy sem_ty_ref sem_ty_prod sem_ty_sum sem_ty_arr sem_ty_aarr sem_ty_uarr sem_ty_forall sem_ty_row_forall sem_ty_exists sem_ty_rec sem_ty_option sem_ty_list.
+Opaque sem_sig_eff sem_sig_flip_bang.
+Opaque sem_row_nil sem_row_flip_bang sem_row_cons sem_row_rec.
 
 Definition C : val := (Λ: Λ: Λ: Λ: λ: "x" "y" "z", ("x" "z") "y")%V.
+Definition C_gen : val := (Λ: C)%V.
 
 Section typing.
 
@@ -42,6 +43,9 @@ Section typing.
 
   Definition C_ms_ty : sem_ty Σ := 
     (∀R: θ, ∀T: α, ∀T: β, ∀T: γ,  (β -{ θ }-∘ ('! α -{ θ }-∘ γ)) → ('! α) ⊸ β -{ θ }-∘ γ)%T.
+
+  Definition C_gen_ty : sem_ty Σ := 
+    (∀M: ν, ∀R: θ, ∀T: α, ∀T: β, ∀T: γ, (β -{ ¡_[ ν ] θ }-∘ ('!_[ν] α -{ ¡_[ ν ] θ }-∘ γ)) → ('!_[ ν ] α) ⊸ β -{ ¡_[ ν ] θ }-∘ γ)%T.
 
   Lemma C_os_typed : ⊢ ⊨ᵥ C : C_os_ty.
   Proof.
@@ -85,6 +89,39 @@ Section typing.
     iApply (sem_typed_app_ms ('! α)); solve_sidecond.
     { iApply sem_typed_app_nil; iApply sem_typed_var'. }
     iApply sem_typed_var'.
+  Qed.
+
+  Lemma C_gen_typed : ⊢ ⊨ᵥ C_gen : C_gen_ty.
+  Proof.
+    iIntros. rewrite /C_gen /C_gen_ty /C.
+    iApply sem_typed_Mclosure; solve_sidecond. iIntros (ν).
+    iApply sem_typed_val. iApply sem_typed_Rclosure; solve_sidecond. iIntros (θ).
+    rewrite - (app_nil_l []).
+    iApply sem_typed_TLam; solve_sidecond. iIntros (α).
+    rewrite - (app_nil_l []).
+    iApply sem_typed_TLam; solve_sidecond. iIntros (β).
+    rewrite - (app_nil_l []).
+    iApply sem_typed_TLam; solve_sidecond. iIntros (γ).
+    rewrite - (app_nil_l []).
+    iApply sem_typed_ufun; solve_sidecond. simpl.
+    rewrite - (app_nil_r [("x", _)]).
+    iApply sem_typed_afun; solve_sidecond. simpl.
+    rewrite - (app_nil_r [("y", _); ("x", _)]).
+    iApply sem_typed_afun; solve_sidecond. simpl.
+    rewrite - (app_nil_r [("y", _); ("x", _)]).
+    iApply (sem_typed_app_gen ('!_[ ν ] α) (¡_[ ν ] θ)%R (¡_[ ν ] θ)%R (¡_[ ν ] θ)%R).
+    - iApply row_le_refl.
+    - iApply row_type_sub_mfbang_mbang.
+    - iApply row_env_sub_copy; solve_copy.
+    - iApply row_le_refl.
+    - iApply (sem_typed_app_gen β (¡ ⟨⟩)%R (¡_[ ν ] θ)%R (¡_[ ν ] θ)%R).
+      + iApply row_le_trans; [iApply row_le_fbang_elim|iApply row_le_nil].
+      + iApply row_type_sub_fbang.
+      + iApply row_env_sub_copy; solve_copy.
+      + iApply row_le_refl.
+      + iApply sem_typed_var'.
+      + iApply sem_typed_var'.
+    - iApply sem_typed_swap_second. iApply sem_typed_var'.
   Qed.
 
 End typing.
