theories/case_studies/cooperative_concurrency_gen.v
@@ -29,9 +29,9 @@ From affect.case_studies Require Import state.
 
 (* Make all the definitions opaque so that we do not rely on their definition in the model to show that the programs are well-typed terms. *)
 Opaque sem_typed sem_typed_val ty_le row_le sig_le row_type_sub row_env_sub.
-Opaque sem_ty_void sem_ty_unit sem_ty_bool sem_ty_int sem_ty_string sem_ty_top sem_ty_cpy sem_env_cpy sem_ty_ref_cpy sem_ty_ref sem_ty_prod sem_ty_sum sem_ty_arr sem_ty_aarr sem_ty_uarr sem_ty_forall sem_ty_row_forall sem_ty_exists sem_ty_rec sem_ty_option sem_ty_list.
-Opaque sem_sig_eff sem_sig_os.
-Opaque sem_row_nil sem_row_os sem_row_tun sem_row_cons sem_row_rec.
+Opaque sem_ty_void sem_ty_unit sem_ty_bool sem_ty_int sem_ty_string sem_ty_top sem_ty_bang sem_env_bang sem_ty_ref_cpy sem_ty_ref sem_ty_prod sem_ty_sum sem_ty_arr sem_ty_aarr sem_ty_uarr sem_ty_forall sem_ty_row_forall sem_ty_exists sem_ty_rec sem_ty_option sem_ty_list.
+Opaque sem_sig_eff sem_sig_flip_bang.
+Opaque sem_row_nil sem_row_flip_bang sem_row_cons sem_row_rec.
 
 Definition impossible : expr := ((rec: "f" <> := "f" #()) #())%E.
 
@@ -253,7 +253,7 @@ Section typing.
     iApply (sem_typed_app_os (Promise ('! ()) ⟨⟩%R)).
     - iApply sem_typed_sub_u2aarr.
       iApply sem_typed_sub_ty; [iApply ty_le_uarr|]; 
-        [iApply row_le_refl|iApply ty_le_refl|iApply ty_le_cpy_elim|].
+        [iApply row_le_refl|iApply ty_le_refl|iApply (ty_le_mbang_elim MS)|].
       iApply sem_typed_sub_nil. simpl. rewrite -/coop.
       set C := (λ θ' α, (Promise ('! α) θ') -{ coop θ' }-> ('! α)).
       rewrite -/(C ⟨⟩%R ()). iApply sem_typed_TApp; first solve_copy.
@@ -269,7 +269,7 @@ Section typing.
       + iApply sem_typed_sub_nil.
         rewrite - {1} (app_nil_r []).
         iApply sem_typed_afun; solve_sidecond. simpl.
-        iApply sem_typed_sub_ty; [iApply ty_le_cpy_intro; solve_copy|].
+        iApply sem_typed_sub_ty; [iApply ty_le_bang_intro; solve_copy|].
         iApply sem_typed_unit'.
   Qed.
 
@@ -523,10 +523,10 @@ Section typing.
            iApply sem_typed_sub_u2aarr.
            iApply sem_typed_sub_ty; first iApply ty_le_uarr; 
             [iApply row_le_refl|iApply ty_le_uarr|iApply ty_le_refl|];
-            [iApply row_le_os_intro|iApply ty_le_refl|iApply ty_le_refl|].
+            [iApply (row_le_mfbang_intro OS)|iApply ty_le_refl|iApply ty_le_refl|].
            iApply sem_typed_sub_ty; first iApply ty_le_uarr; 
             [iApply row_le_refl|iApply ty_le_refl|iApply ty_le_aarr|];
-            [iApply row_le_os_elim|iApply ty_le_refl|iApply ty_le_refl|].
+            [iApply row_le_fbang_elim|iApply ty_le_refl|iApply ty_le_refl|].
             set C := (λ (θ : sem_row Σ), (('! β -{ θ' }-∘ ()) -{ ¡ θ }-> ()) → List ('! β -{θ'}-∘ ()) -{ ¡ θ }-∘ ())%T.
            rewrite -/(C ⊥).
            iApply sem_typed_RApp; first solve_copy. 
@@ -564,8 +564,8 @@ Section typing.
     iApply (sem_typed_app_nil (() -{ coopstate }-∘ ())).
     - iApply sem_typed_sub_ty; first iApply ty_le_u2aarr.
       iApply sem_typed_sub_ty.
-      { iApply ty_le_uarr; [iApply row_le_refl| |iApply ty_le_cpy_elim].
-        iApply ty_le_aarr; [iApply row_le_refl|iApply ty_le_refl|iApply ty_le_cpy_intro; solve_copy]. }
+      { iApply ty_le_uarr; [iApply row_le_refl| |iApply (ty_le_mbang_elim MS)].
+        iApply ty_le_aarr; [iApply row_le_refl|iApply ty_le_refl|iApply ty_le_bang_intro; solve_copy]. }
       set R := (λ α θ', (() -{ coop θ' }-∘ '! α) -{ θ' }-> '! α)%T.
       rewrite /coopstate -/(R () st).
       iApply (sem_typed_RApp (R ())).
@@ -597,7 +597,7 @@ Section typing.
           rewrite -/(coop st) {1} /coop_pre {7} /st.
           iApply sem_typed_sub_row; first iApply row_le_swap_third; try done.
           iApply sem_typed_sub_row; first iApply row_le_swap_second; try done.
-          iApply sem_typed_sub_ty; first iApply ty_le_cpy_intro; first solve_copy.
+          iApply sem_typed_sub_ty; first iApply ty_le_bang_intro; first solve_copy.
           iApply (sem_typed_perform_ms (TT:=[tele _]) [tele_arg ()] with "[] []"); solve_sidecond.
           iApply sem_typed_sub_row; first iApply row_le_swap_fourth; try done.
           do 2 (iApply sem_typed_sub_row; first iApply row_le_swap_third; try done).
@@ -607,7 +607,7 @@ Section typing.
         * set A := (λ α θ', Promise ('! α) θ' -{ coop θ' }-> '! α)%T.
           iApply (sem_typed_app_nil p1type).
           { iApply sem_typed_sub_ty; first iApply ty_le_u2aarr.
-            iApply sem_typed_sub_ty; first iApply ty_le_uarr; [iApply row_le_refl|iApply ty_le_refl|iApply ty_le_cpy_elim| ].
+            iApply sem_typed_sub_ty; first iApply ty_le_uarr; [iApply row_le_refl|iApply ty_le_refl|iApply (ty_le_mbang_elim MS)| ].
             rewrite /coopstate /p1type -/(A () st).
             iApply (sem_typed_TApp (λ α, A α st)).
             iApply (sem_typed_RApp (λ θ', ∀T: α, A α θ')).
